\item 
\begin{enumerate}

\item
\begin{itemize}
\item $\frac{x+6}{x^2-4} = \frac{A}{x-2}+\frac{B}{x+2}$
\item $\frac{x+6}{x^2-4} = \frac{(A+B)x+(2A-2B)}{(x-2)(x+2)}$
\item $A+B=1$ und $2A-2B=6$
\item $B=-1$ und $A=2$
\end{itemize}

\item 
\begin{itemize}
\item $2y\dd{x}{y} = \frac{2}{x-2} - \frac{1}{x+2}$
\item $\int 2y \diff{y} = \int \frac{2}{x-2} - \frac{1}{x+2} \diff{x}$
\item $y^2 = 2\ln(|x-2|) - \ln(|x+2|) + C$
\item $y(x) = \pm \sqrt{2\ln(|x-2|) - \ln(|x+2|) + C}$
\end{itemize}

\end{enumerate}
