\item
\begin{enumerate}

\item
\begin{itemize}
\item $p_2 =
1\cdot\frac{x-1}{0-1}\cdot\frac{x-2}{0-2} +
3\cdot\frac{x-0}{1-0}\cdot \frac{x-2}{1-2} +
7\cdot\frac{x-0}{2-0}\cdot\frac{x-1}{2-1}$
\item $=\frac{1}{2}(x-1)(x-2)-3x(x-2)+\frac{7}{2}x(x-1)$
\item $=\frac{1}{2}(x^2-3x+2)-3(x^2-2x)+\frac{7}{2}(x^2-x)$
\item $=(\frac{1}{2}-3+\frac{7}{2})x^2+(-\frac{3}{2}+6-\frac{7}{2})x+2\cdot\frac{1}{2}$
\item $=x^2+x+1$
\end{itemize}

\item
\begin{itemize}
\item $p_2(x_2) =
y_1\cdot\underbrace{\frac{x_2-x_2}{x_1-x_2}}_0\cdot\frac{x_2-x_3}{x_1-x_3} +
y_2\cdot\underbrace{\frac{x_2-x_1}{x_2-x_1}}_1\cdot\underbrace{\frac{x_2-x_3}{x_2-x_3}}_1 +
y_3\cdot\frac{x_2-x_1}{x_3-x_1}\cdot\underbrace{\frac{x_2-x_2}{x_3-x_2}}_0$
\item $=y_2$
\end{itemize}

\end{enumerate}
