\item
	\begin{enumerate}
	
	\item Partielle Ableitung sind unabh√§ngig der Reihenfolge, in der nach Variablen abgeleitet wird
		\begin{itemize}
			\item $f_{ab} = f_{ba}$
			\item $f_{ac} = f_{ca}$
			\item $f_{abc} = f_{cba}$
		\end{itemize}
	
	\item
		\begin{itemize}
			\item $ f_a = \frac{3a^2\sin(-3b)}{2c}$
			\item $ f_{ab}= \frac{3a^2\cdot (-3) \cdot \cos(-3b)}{2c}$
			\item $ f_{ab}= \frac{-9a^2\cdot \cos(-3b)}{2c}$
			\item $ f_{abc}= -\frac{-9a^2\cdot \cos(-3b)}{2c^2}$
			\item $ f_{abc}= \frac{9a^2\cdot \cos(-3b)}{2c^2} = \frac{9a^2\cdot \cos(3b)}{2c^2}$
		\end{itemize}
		
	\end{enumerate}
