\item
\begin{enumerate}
\item $f_x = -\frac{1}{x}$, $f_y = \frac{1}{y}$
\item $f_x = \frac{-e^{x-y}}{2-e^{x-y}} = \frac{-e^{-y}e^x}{-e^{-y}(-2e^y+e^x)} = \frac{e^x}{e^x-2e^y}$, $f_y = \frac{e^{x-y}}{2-e^{x-y}} = -\frac{e^x}{e^x-2e^y}$
\item $f_x = 2y\cdot x^{2y-1}$, $f_y = 2\ln(x)x^{2y}$
\item $f_x = -y \cdot \sin(e^{xy}+xy) \cdot (e^{xy}+1)$, $f_y = -x \cdot \sin(e^{xy}+xy) \cdot (e^{xy}+1)$ 
\item $f_x = (y-x) \cdot (1-2xy+x^2)^{-\frac{3}{2}}$, $f_y = x \cdot (1-2xy+x^2)^{-\frac{3}{2}}$
\item $f_x = \frac{1}{x\ln(y)}$, $f_y=-\frac{\ln(x)}{y\ln(y)^2}$
\end{enumerate}

