\item
\begin{enumerate}

\item $\frac{\d{}}{\d x} \lbrack \sin((x+3)^2) \rbrack = 2(x+3)\cos((x+3)^2)$

\item

$\frac{\d{}}{\d x} \lbrack \sin(\sqrt x) \rbrack$

$=\frac{1}{2}(\cos(\sqrt x)x^{-\frac{1}{2}}$

$=\frac{1}{2\sqrt{x}}(\cos(\sqrt x)$

\item

$\frac{\d{}}{\d x} \lbrack (e^x \ln(x))^3 \rbrack $

$\stackrel{\text{Kettenregel}}{=} 3(e^x\ln(x))^2 \cdot \frac{\d{}}{\d x}[e^x\ln(x)]$

$\stackrel{\text{Produktregel}}{=} 3e^{2x}(\ln(x))^2(e^x\ln(x)+\frac{e^x}{x})$

$\stackrel{\text{ausklammern}}{=} 3e^{3x}(\ln(x))^2(\ln(x)+\frac{1}{x})$
\end{enumerate}

