\item

\begin{enumerate}
\item $\int\limits_2^5 \frac{1}{(x-3)^2}\diff{x} = \int\limits_{-1}^2 \frac{1}{x^2} \diff{x} \stackrel{\text{def}}{=} \lim\limits_{\varepsilon\to 0^{+}} (\int\limits_{-1}^{-\varepsilon} \frac{1}{x^2} \diff{x} + \int\limits_{\varepsilon}^5 \frac{1}{x^2}\diff{x}) = \lim\limits_{\varepsilon\to 0^{+}} (\frac{2}{\varepsilon} - \frac{3}{2})$

Dieser Grenzwert konvergiert nicht, daher hat das uneigentliche Integral keinen Hauptwert.

\item $\int\limits_2^3 \frac{1}{\sqrt{x-2}}\diff{x} = \int\limits_0^1 \frac{1}{\sqrt{x}}\diff{x} \stackrel{\text{def}}{=} \lim\limits_{\varepsilon\to 0^{+}} \int\limits_\varepsilon^1 \frac{1}{\sqrt{x}} = \lim\limits_{\varepsilon\to 0^{+}}(2-2\sqrt{\varepsilon}) = 2$
\end{enumerate}

