\item

\begin{enumerate}
\item $\int\limits_2^5 \frac{1}{(x-3)^2}\d x = \int\limits_{-1}^2 \frac{1}{x^2} \d x \stackrel{\text{def}}{=} \lim\limits_{\epsilon\to 0^{+}} (\int\limits_{-1}^{-\epsilon} \frac{1}{x^2} \d x + \int\limits_{\epsilon}^5 \frac{1}{x^2}\d x) = \lim\limits_{\epsilon\to 0^{+}} (\frac{2}{\epsilon} - \frac{3}{2})$

Dieser Grenzwert konvergiert nicht, daher hat das uneigentliche Integral keinen Hauptwert.

\item $\int\limits_2^3 \frac{1}{\sqrt{x-2}}\d x = \int\limits_0^1 \frac{1}{\sqrt{x}}\d x \stackrel{\text{def}}{=} \lim\limits_{\epsilon\to 0^{+}} \int\limits_\epsilon^1 \frac{1}{\sqrt{x}} = \lim\limits_{\epsilon\to 0^{+}}(2-2\sqrt{\epsilon}) = 2$
\end{enumerate}

