\item

\begin{enumerate}
\item $\lim\limits_{x \to \infty} \frac{3}{x} = 0$ (Hyperbel)
\item $\lim\limits_{x \to \infty} \frac{2x-5}{4} = \infty$ (lineare Funktion mit positiven Anstieg)
\item $\lim\limits_{x\to 3} e^{(x^2)} \stackrel{\text{Einsetzen}}{=} e^{(3^2)} = e^9$
\item $\lim\limits_{v\to 3} \frac{e^{v-3}-1}{v-3} = \lim\limits_{x\to 0}\frac{e^{x}-1}{x} \stackrel{\text{l'Hôpital}}{=} \lim\limits_{x\to 0} \frac{e^x}{1} = 1$
\item $\lim\limits_{x\to 3}\frac{x^2-6x+9}{x^3-3x^2-9x+27} \stackrel{\text{l'Hôpital}}{=} \lim\limits_{x\to 3}\frac{2x-6}{3x^2-6x-9} \stackrel{\text{l'Hôpital}}{=} \lim\limits_{x\to 3}\frac{2}{6x-6} = \frac{2}{18-6} = \frac{2}{12} = \frac{1}{6} $
\item $\lim\limits_{x\to e}\frac{x}{e \cdot (\ln(x^2)-1)} \stackrel{\text{Einsetzen}}{=} \frac{e}{e\cdot(2-1)} = 1$
\end{enumerate}

